And3 working again.

Inserters/And3.dfy
@@ -6,98 +6,304 @@ module Inserters.And3{
   import opened Eval
   import opened ConservedSubcircuit
   import opened Utils
-  import opened Entity
+  import opened Scuf
   import opened MapFunction
   import opened ConnectionEval
   import opened Connection
-  import opened IslandBundle
   import opened Subcircuit
   import opened MapConnection
+  import opened Modifiers.Merge
+  import opened SelfConnect
+  import opened Modifiers.Connect
+  import opened Path
+  import opened Modifiers.SwitchUF
+  import opened Modifiers.NewOutputs
 
   import opened And
 
-  function InsertAnd3Impl(c: Circuit): (r: (Circuit, Entity))
-    requires c.Valid()
-    ensures r.0.Valid()
-    ensures EntityValid(r.0, r.1)
+  const And3UFConst := UpdateFunction(
+    3, 1, 0,
+    (si: SI) requires |si.inputs| == 3 && |si.state| == 0 =>
+      SO([si.inputs[0] && si.inputs[1] && si.inputs[2]], []))
+
+  function And3UF(): (r: UpdateFunction)
+    ensures r.Valid()
   {
-    reveal SimpleInsertion();
+    reveal UpdateFunction.Valid();
+    And3UFConst
+  }
 
-    var eb1 := IslandBundleFromCircuit(c);
-    var (c1, e1) := InsertAnd(c);
-    var (eb2, a_ref) := AddEntity(eb1, c1, e1);
-    assert e1.sc == {e1.mf.outputs[0].n};
-    assert EntityValid(c1, e1);
+  function And3Step1UF(): (r: UpdateFunction)
+    ensures r.Valid()
+  {
+    reveal UpdateFunction.Valid();
+    UpdateFunction(
+    4, 2, 0,
+    (si: SI) requires |si.inputs| == 4 && |si.state| == 0 =>
+      SO([si.inputs[0] && si.inputs[1], si.inputs[2] && si.inputs[3]], []))
+  }
+  
+  function And3Step1UFx(): (r: UpdateFunction)
+  ensures r.input_width == 4
+  ensures r.output_width == 2
+  ensures r.state_width == 0
+  {
+    reveal MergeUpdateFunctions();
+    MergeUpdateFunctions(AndUF(), AndUF())
+  }
 
-    assert e1 == eb2.es[a_ref].value;
+  function And3Step1SF(si: SI): (so: SO)
+    requires |si.inputs| == 4
+    requires |si.state| == 0
+  {
+    MergeSF(AndUF(), AndUF(), si)
+  }
 
-    var (c2, e2) := InsertAnd(c1);
-    var (eb3, b_ref) := AddEntity(eb2, c2, e2);
-    assert e2.sc == {e2.mf.outputs[0].n};
+  lemma {:vcs_split_on_every_assert} LemmaAnd3Step1UF()
+    ensures UpdateFunctionsEquiv(And3Step1UF(), And3Step1UFx())
+  {
+    var uf1 := And3Step1UF();
+    var ufa := AndUF();
+    var uf2 := MergeUpdateFunctions(ufa, ufa);
+    assert uf2.input_width == 4 by {reveal MergeUpdateFunctions();}
+    assert uf2.output_width == 2 by {reveal MergeUpdateFunctions();}
+    assert uf2.state_width == 0 by {reveal MergeUpdateFunctions();}
 
-    assert e1 == eb3.es[a_ref].value;
-    assert EntityValid(eb3.c, e1) && IsIsland(eb3.c, e1.sc) by {
-      reveal IslandBundleValid();
+    forall si: SI | uf1.SIVal(si)
+      ensures uf2.sf.requires(si)
+      ensures uf1.sf(si) == uf2.sf(si)
+    {
+      assert uf2.sf.requires(si) && uf2.sf(si) == MergeSF(ufa, ufa, si) by {
+        reveal MergeUpdateFunctions();
+      }
+      reveal UpdateFunction.Valid();
+      assert uf1.sf(si) == uf2.sf(si);
     }
+    reveal UpdateFunctionsEquiv();
+  }
 
-    var a_i0 := e1.mf.inputs[0];
-    var a_i1 := e1.mf.inputs[1];
-    var a_o := e1.mf.outputs[0];
+  function And3Step2UF(): (r: UpdateFunction)
+    ensures r.Valid()
+  {
+    reveal UpdateFunction.Valid();
+    UpdateFunction(
+    3, 2, 0,
+    (si: SI) requires |si.inputs| == 3 && |si.state| == 0 =>
+      SO([si.inputs[0] && si.inputs[1], si.inputs[0] && si.inputs[1] && si.inputs[2]], []))
+  }
 
-    var b_i0 := e2.mf.inputs[0];
-    var b_i1 := e2.mf.inputs[1];
-    var b_o := e2.mf.outputs[0];
+  function And3Step2UFx(): (r: UpdateFunction)
+  {
+    var conn := And3InternalConnection();
+    ConnectUpdateFunction(And3Step1UFx(), conn)
+  }
 
-    var i0 := a_i0;
-    var i1 := a_i1;
-    var i2 := b_i0;
-    var o := b_o;
+  lemma LemmaAnd3Step2UF()
+    ensures
+      var conn := And3InternalConnection();
+      UpdateFunctionsEquiv(And3Step2UF(), And3Step2UFx())
+  {
+    LemmaAnd3Step1UF();
+    reveal UpdateFunctionsEquiv();
+  }
 
-    var combined_inputs := [i0, i1, i2];
-    var combined_outputs := [o];
+  function And3Step3UF(): (r: UpdateFunction)
+    ensures r.Valid()
+  {
+    reveal UpdateFunction.Valid();
+    UpdateFunction(
+    3, 1, 0,
+    (si: SI) requires |si.inputs| == 3 && |si.state| == 0 =>
+      SO([si.inputs[0] && si.inputs[1] && si.inputs[2]], []))
+  }
 
-    var combined_mf := MapFunction(combined_inputs, combined_outputs, [],
-      (si: SI) requires SIValid(si, combined_inputs, []) =>
-      reveal Seq.ToSet();
-      SO([si.inputs[0] && si.inputs[1] && si.inputs[2]], [])
-    );
-    assert combined_mf.Valid() by {
-      reveal Seq.ToSet();
-      reveal Seq.HasNoDuplicates();
-      reveal MapFunction.Valid();
-    }
-    var combined_e := Entity(e1.sc + e2.sc, combined_mf);
+  function And3Step3UFx(): (r: UpdateFunction)
+  {
+    var new_outputs := And3NewOutputs();
+    NewOutputsUpdateFunction(And3Step2UFx(), new_outputs)
+  }
 
-    var abiaobi: seq<(bool, nat)> := [(false, 2), (true, 0)];
-    var aoboabo: seq<(bool, nat)> := [(true, 0)];
-    assert MakeConnectionsReqs(e1.mf, e2.mf, combined_mf, [0, 1], abiaobi, aoboabo, [], [], []) by {
-      reveal Seq.HasNoDuplicates();
-      reveal ConnectionX<NP>.Valid();
-      reveal ConnectionX<CNode>.Valid();
-      reveal ConnectionXY<NP>.Valid();
-      reveal ConnectionXY<CNode>.Valid();
-    }
-    var conn := MakeConnections(e1.mf, e2.mf, combined_mf, [0, 1], abiaobi, aoboabo, [], [], []);
-    assert conn.SomewhatValid();
+  lemma LemmaAnd3Step3UF()
+    ensures
+      UpdateFunctionsEquiv(And3Step3UF(), And3Step3UFx())
+  {
+    LemmaAnd3Step2UF();
+    reveal UpdateFunctionsEquiv();
+  }
+
+  lemma And3UpdateFunctionsEquiv()
+    ensures 
+      reveal MergeUpdateFunctions();
+      var merged_uf := MergeUpdateFunctions(AndUF(), AndUF());
+      var conn := And3InternalConnection();
+      var connected_uf := ConnectUpdateFunction(merged_uf, conn);
+      var new_outputs := And3NewOutputs();
+      var new_outputs_uf := NewOutputsUpdateFunction(connected_uf, new_outputs);
+      UpdateFunctionsEquiv(And3UF(), new_outputs_uf)
+  {
+      LemmaAnd3Step3UF();
+      reveal UpdateFunctionsEquiv();
+  }
+
+  function And3InternalConnection(): (r: InternalConnection)
+    ensures r.Valid()
+    ensures r.connections.Keys == {3}
+    ensures r.connections.Values == {0}
+  {
+    var ni_width := 3;
+    var i_width := 4;
+    var o_width := 2;
+    var connections := map[3 := 0];
+    var i2ni := [0, 1, 2];
+    var nio2i := [(false, 0), (false, 1), (false, 2), (true, 0)];
+    var conn := InternalConnection(ni_width, i_width, o_width, connections, i2ni, nio2i);
     assert conn.Valid() by {
+      reveal InternalConnection.Valid();
       reveal Seq.HasNoDuplicates();
-      reveal MapFunction.Valid();
-      reveal Seq.ToSet();
-      reveal conn.SeqEvaluatesCorrectly();
+    }
+    conn
+  }
+
+  function And3NewOutputs(): (r: seq<nat>)
+    ensures Seq.HasNoDuplicates(r)
+  {
+    reveal Seq.HasNoDuplicates();
+    [1]
+  }
+
+  lemma And3ScufConnectionConsistent(c: Circuit)
+    requires c.Valid()
+    ensures
+      var z_and1 := AndInserter();
+      var z_and2 := AndInserter();
+      var z := MergeModifier(z_and1, z_and2);
+      var (new_c, s) := z.fn(c);
+      var conn := And3InternalConnection();
+      && new_c.Valid()
+      && s.Valid(new_c)
+      && ScufConnectionConsistent(new_c, s, conn)
+  {
+    reveal Seq.ToSet();
+
+    var z_and1 := AndInserter();
+    var z_and2 := AndInserter();
+    assert z_and1.uf.input_width == 2;
+    var z := MergeModifier(z_and1, z_and2);
+    MergeModifierPathConstraints(z_and1, z_and2, c);
+    var (new_c, s) := z.fn(c);
+
+    var conn := And3InternalConnection();
+    assert conn.connections == map[3 := 0];
+    assert conn.connections.Keys == {3};
+    assert conn.connections.Values == {0};
+
+    assert forall index :: index in conn.connections.Values ==> index < 1;
+
+    assert new_c.Valid() && s.Valid(new_c) by {
+      reveal ScufInserter.Valid();
+      reveal SimpleInsertion();
+      z.ValidForCircuit(c);
+      assert SimpleInsertion(c, new_c, s);
+    }
+  
+    reveal InternalConnection.Valid();
+    reveal ONPsValid();
+    s.SomewhatValidToRelaxInputs(new_c);
+    ScufFOutputsAreValid(new_c, s);
+    assert s.uf.input_width == 4 && s.uf.output_width == 2 by {
+      reveal MergeInserter();
+    }
+    var conn_outputs := conn.GetConnectedOutputs(s.mp);
+    assert conn_outputs == {s.mp.outputs[0]};
+    var conn_inputs := conn.GetConnectedInputs(s.mp);
+    assert conn_inputs == {s.mp.inputs[3]};
+
+    assert ScufConnectionConsistent(new_c, s, conn) by {
+      reveal InternalConnection.Valid();
+      reveal ONPsValid();
+      s.SomewhatValidToRelaxInputs(new_c);
+      ScufFOutputsAreValid(new_c, s);
+      assert s.uf.input_width == 4 && s.uf.output_width == 2 by {
+        reveal MergeInserter();
+      }
+      assert (conn.i_width == s.uf.input_width);
+      assert (conn.o_width == s.uf.output_width);
+      var s1_inputs := Seq.ToSet(s.mp.inputs[..z_and1.uf.input_width]);
+      assert s1_inputs == {s.mp.inputs[0], s.mp.inputs[1]};
+      var s2_inputs := Seq.ToSet(s.mp.inputs[z_and1.uf.input_width..]);
+      assert s2_inputs == {s.mp.inputs[2], s.mp.inputs[3]};
+      var s1_outputs := Seq.ToSet(s.mp.outputs[..z_and1.uf.output_width]);
+      assert s1_outputs == {s.mp.outputs[0]};
+      var s2_outputs := Seq.ToSet(s.mp.outputs[z_and1.uf.output_width..]);
+      assert s2_outputs == {s.mp.outputs[1]};
+      assert !PathExistsBetweenNPSets(new_c, s1_outputs, s2_inputs);
+      assert conn.GetConnectedOutputs(s.mp) <= s1_outputs;
+      assert conn.GetConnectedInputs(s.mp) <= s2_inputs;
+      NoPathExistsBetweenNPSubSets(new_c, s1_outputs, s2_inputs, conn.GetConnectedOutputs(s.mp), conn.GetConnectedInputs(s.mp));
+      assert !PathExistsBetweenNPSets(new_c, conn.GetConnectedOutputs(s.mp), conn.GetConnectedInputs(s.mp));
+      assert Seq.ToSet(s.mp.inputs) !! new_c.PortSource.Keys by {
+        reveal ScufInserter.Valid();
+        assert z.SpecificValid(c);
+        reveal SimpleInsertion();
+        assert IsIsland(new_c, s.sc);
+        InputsOfIslandNotInPortSource(new_c, s);
+      }
+      assert (forall i_index :: i_index in conn.connections ==> s.mp.inputs[i_index] !in new_c.PortSource);
+      reveal ScufConnectionConsistent();
+    }
+  }
+
+  opaque function And3Inserter(): (z: ScufInserter)
+    ensures z.Valid()
+  {
+    reveal Seq.ToSet();
+
+    var z_and1 := AndInserter();
+    var z_and2 := AndInserter();
+    assert z_and1.uf.input_width == 2;
+
+    reveal MergeUpdateFunctions();
+    var z_par_ands := MergeModifier(z_and1, z_and2);
+    assert z_par_ands.uf.input_width == 4;
+
+    var conn := And3InternalConnection();
+
+    assert InserterConnectionConsistent(z_par_ands, conn) by {
+      assert UFConnectionConsistent(z_par_ands.uf, conn) by {
+        assert (conn.i_width == z_par_ands.uf.input_width);
+        assert (conn.o_width == z_par_ands.uf.output_width);
+      }
+      forall c: Circuit | c.Valid()
+        ensures
+          var (new_c, s) := z_par_ands.fn(c);
+          && new_c.Valid() && s.Valid(new_c)
+          && ScufConnectionConsistent(new_c, s, conn)
+      {
+        var (new_c, s) := z_par_ands.fn(c);
+        And3ScufConnectionConsistent(c);
+        assert ScufConnectionConsistent(new_c, s, conn);
+      }
+      reveal InserterConnectionConsistent();
     }
 
-    IsIslandInputsNotInPortSource(eb3.c, e2);
-    assert ConnectEntitiesRequirements(eb3.c, e1, e2, combined_e, conn);
-    var (eb4, ab_ref) := IBConnectEntities(eb3, a_ref, b_ref, combined_e, conn);
-    var e_ab := eb4.es[ab_ref].value;
-    assert eb4.es == [None, None, Some(e_ab)];
+    var z_connected := ConnectModifier(z_par_ands, conn);
+    assert z_connected.Valid();
 
-    assert IsIsland(eb4.c, e_ab.sc) by {
-      reveal IslandBundleValid();
+
+    var new_outputs := And3NewOutputs();
+    var z_remove_outputs := NewOutputsModifier(z_connected, new_outputs);
+
+    var merged_uf := MergeUpdateFunctions(AndUF(), AndUF());
+    var connected_uf := ConnectUpdateFunction(merged_uf, conn);
+    var final_uf := NewOutputsUpdateFunction(connected_uf, new_outputs);
+    assert connected_uf == z_connected.uf;
+    assert final_uf == z_remove_outputs.uf;
+
+    assert UpdateFunctionsEquiv(And3UF(), final_uf) by {
+      And3UpdateFunctionsEquiv();
     }
-    assert IsIsland(eb4.c, e_ab.sc);
-    IsIslandNoOutputs(eb4.c, e_ab.sc);
-    (eb4.c, e_ab)
+    var z_switched := SwitchUFModifier(z_remove_outputs, And3UF());
+    z_switched
   }
 
 }
